Negace výroků:
\begin{multicols}{2}
\begin{enumerate}
	\item  $\neg (\neg A) \equiv A$
	\item  $\neg (A \wedge B) \equiv (\neg A) \vee (\neg B)$
	\item  $\neg (A \vee B) \equiv (\neg A) \wedge (\neg B)$
	\item  $\neg (A \Rightarrow B) \equiv A \wedge (\neg B)$
	\item  $\neg (A \Leftrightarrow B) \equiv A \Leftrightarrow (\neg B)$
	\item  $\neg \left( \forall x \colon \varphi(x) \right) \equiv \exists x \colon \neg \varphi(x)$
	\item  $\neg \left( \exists x \colon \varphi(x) \right) \equiv \forall x \colon \neg \varphi(x)$
\end{enumerate}
\end{multicols}
Pozor na ``existuje právě jedno'': $\neg \left( \exists! x \colon \varphi(x) \right) \equiv \left( \forall x \colon \neg \varphi(x) \right) \vee \left( \exists x \exists y \colon x \neq y \wedge \varphi(x) \wedge \varphi(y) \right)$

